\paragraph{Sum}
\begin{align*}
	\sum_{i=1}^n i^2 &= \frac{1}{6}n(n+1)(2n+1) \\
	\sum_{i=1}^n i^3 &= \Big[\frac{n(n+1)}{2}\Big]^2 \\
	\sum_{i=1}^n i^4 &= \frac{6n^5+15n^4+10n^3-n}{30} \\
	\sum_{i=1}^n i^5 &= \frac{2n^6+6n^5+5n^4-n^2}{12} 
\end{align*}

\paragraph{Fibonacci}
\[ F_n=\begin{cases}
	0 & n=0 \\
	1 & n=1 \\
	F_{n-1}+F_{n-2} & n \geq 2 \\
\end{cases} \]
\[ F_n=\frac{1}{\sqrt{5}}\Big[\Big(\frac{1+\sqrt{5}}{2}\Big)^n-\Big(\frac{1-\sqrt{5}}{2}\Big)^n\Big] \]

\paragraph{Catalan}
\[ C_n=\begin{cases}
	0 & n=0 \\
	\sum\limits_{i=0}^{n-1} C_i C_{n-1-i} & n \geq 1 \\
\end{cases} \]
\[ C_n= \Big(\begin{array}{c} 2n\\n \end{array} \Big) - \Big(\begin{array}{c} 2n\\(n+1) \end{array} \Big) = \frac{1}{n+1}\Big(\begin{array}{c} 2n\\n \end{array} \Big) \]

\paragraph{错排}
\[ D_n=\begin{cases}
	0 & n=1 \\
	1 & n=2 \\
	(n-1)(D_{n-1}+D_{n-2}) & n \geq 2 \\
\end{cases} \]
\[ D_n=n!\Big(1-\frac{1}{1!}+\frac{1}{2!}-\frac{1}{3!}+ \dots +(-1)^n\frac{1}{n!} \Big) \]

